More DarkForest and Semaphore

dsl/circuits/darkforest/darkforest.ml
@@ -106,8 +106,7 @@ let quin_selector =
 
 (* IsNegative *)
 
-(* TODO: Need integer division to specify this correctly *)
-let t_is_neg = tf
+let t_is_neg = tfq (ind_dec nu (lt (toSZ vin) z0))
 
 let is_neg =
   Circuit
@@ -115,7 +114,7 @@ let is_neg =
     ; inputs= [("in", tf)]
     ; outputs= [("out", t_is_neg)]
     ; dep= None
-    ; body= elet "z" (call "Num2Bits" [z254; vin]) (call "Sign" [z]) }
+    ; body= elet "z" (call2 "Num2Bits" z254 vin) (call1 "Sign" z) }
 
 (* Random *)
 
